tmp

Snlean/lambda.lean
@@ -22,7 +22,7 @@ def type_env := List (Nat × type)
 inductive has_type : type_env → term → type → Prop
 | var_rule : ∀ (gamma : type_env) (x : Nat) (t : type), gamma.elem (x, t) → has_type gamma (var x) t
 | abs_rule : ∀ (gamma : type_env) (x : Nat) (t1 t2 : type) (e : term), has_type ((x, t1) :: gamma) e t2 → has_type gamma (abs t1 e) (type.arrow t1 t2)
-| app_rule : ∀ (gamma : type_env) (e1 e2 : term) (t2 t1 : type), has_type gamma e1 (type.arrow t2 t1) → has_type gamma e2 t2 → has_type gamma (app e1 e2) t1
+| app_rule : ∀ (gamma : type_env) (e1 e2 : term) (t1 t2 : type), has_type gamma e1 (type.arrow t2 t1) → has_type gamma e2 t2 → has_type gamma (app e1 e2) t1
 open has_type
 
 inductive value : term → Prop
@@ -43,56 +43,67 @@ open eval
 theorem env_var_rule_noemp : ∀ (x : Nat) (T : type) (gamma : type_env), has_type gamma (var x) T → gamma ≠ [] := by
   intro x T gamma ht env_is_emp;
   cases ht with
-  | var_rule _ _ _ env_is_not_emp =>
-    rw [env_is_emp] at env_is_not_emp
+  | var_rule _ _ _ env_isnt_emp =>
+    rw [env_is_emp] at env_isnt_emp
     contradiction
 
 theorem progress : ∀ (t : term) (T : type) (gamma : type_env), has_type gamma t T ∧ gamma = [] → value t ∨ (∃t' : term, eval t t') := by
-  intro t T gamma ht;
-  have t_wt := And.left ht;
-  have env_is_emp := And.right ht;
+  intro t T gamma premise;
+  have t_wt := And.left premise;
+  have env_is_emp := And.right premise;
   induction t_wt with
-  | var_rule _ _ _ pre =>
-    rw [env_is_emp] at pre
+  | var_rule _ _ _ x_elem_env =>
+    -- Contradictory because env_is_emp contradicts x_elem_env
+    rw [env_is_emp] at x_elem_env
     contradiction
   | abs_rule =>
+    -- Straightforward because t is value
     apply Or.intro_left
     apply value.abs
-  | app_rule gamma e1 e2 T1 T2 pre1 pre2 ihe1 ihe2 =>
+  | app_rule gamma e1 e2 T1 T2 wte1 wte2 ihe1 ihe2 =>
     cases e1 with
     | var x =>
-      have env_is_not_emp := env_var_rule_noemp x (arrow T1 T2) gamma pre1
+      -- Contradictory because env is emp
+      have env_isnt_emp := env_var_rule_noemp x (arrow T2 T1) gamma wte1
       contradiction
     | abs _ _ =>
       cases e2 with
       | var x =>
-        have env_is_not_emp := env_var_rule_noemp x T1 gamma pre2
+        -- Contradictory because env is emp
+        have env_isnt_emp := env_var_rule_noemp x T2 gamma wte2
         contradiction
       | abs _ _ =>
+        -- (\x. t) v -> [x \mapsto v] t
         apply Or.intro_right
         apply Exists.intro
         apply e_app_abs
         apply value.abs
       | app _ _ =>
+        -- t2 -> t2' implies
+        -- (\x. t1) t2 -> (\x. t1) t2'
         apply Or.intro_right
-        have r := And.intro pre2 env_is_emp;
-        cases ihe2 r env_is_emp with
-        | inl h1 =>
+        cases ihe2 (And.intro wte2 env_is_emp) env_is_emp with
+        | inl _ =>
+          -- Straightforward because app _ _ is not a value
           contradiction
-        | inr h2 =>
-          cases h2 with
+        | inr ihe2_cons_exists =>
+          -- Applying ih
+          cases ihe2_cons_exists with
           | intro _ h =>
             apply Exists.intro
             apply e_app_right
             apply value.abs
             apply h
     | app _ _ =>
+      -- t1 -> t1' implies
+      -- t1 t2 -> t1' t2
       apply Or.intro_right
-      have r := And.intro pre1 env_is_emp;
-      cases ihe1 r env_is_emp with
+      cases ihe1 (And.intro wte1 env_is_emp) env_is_emp with
       | inl h1 =>
+        -- Straightforward because app _ _ is not a value
         contradiction
       | inr h2 =>
+        -- Applying ih
         cases h2 with
         | intro _ h =>
           apply Exists.intro
@@ -103,29 +114,27 @@ theorem subst_preservation : ∀ (s t : term) (x : Nat) (S T : type) (gamma : ty
   has_type gamma s S → has_type (List.cons (x, S) gamma) t T → has_type gamma (subst t x s) T := by
   sorry
 
-theorem preservation : ∀ (e e' : term) (t : type) (gamma : type_env),
-  has_type gamma e t → eval e e' → has_type gamma e' t := by
-  intro e e' t gamma ht ev;
-  induction ht with
+theorem preservation : ∀ (e e' : term) (T : type) (gamma : type_env),
+  has_type gamma e T → eval e e' → has_type gamma e' T := by
+  intro e e' T gamma wte ev;
+  induction wte with
   | var_rule _ _ _ pre =>
+    -- Contradictory to ev bacause var cannot be evaluated
     contradiction
   | abs_rule =>
+    -- Contradictory to ev bacause abs is a value and no rules evaluate it
     contradiction
-  | app_rule gamma e1 e2 T1 T2 pre1 pre2 ih1 ih2 =>
+  | app_rule gamma e1 e2 T1 T2 wte1 wte2 ihe1 ihe2 =>
     cases ev with
-    | e_app_abs T e v vv =>
-      cases vv with
-      | abs T b =>
-        apply subst_preservation e b T T1
-    | e_app_left e1 e1' e2' ev1 =>
-      apply has_type.app_rule
+    -- e_app_abs : ∀ (t : type) (e v : term), value v → eval (app (abs t e) v) (subst e 0 v)
+    | e_app_abs T e v v_is_value =>
+      sorry
+    -- e_app_left : ∀ (e1 e1' e2 : term), eval e1 e1' → eval (app e1 e2) (app e1' e2)
+    | e_app_left e1 e1' e2' eve1 =>
+      apply app_rule
       apply ihe1
-      assumption
-      assumption
-      assumption
-    | e_app_right v e2 e2' vv ev2 =>
+    -- e_app_right : ∀ (v e2 e2' : term), value v → eval e2 e2' → eval (app v e2) (app v e2')
+    | e_app_right v e2 e2' v_is_value eve2 =>
       apply has_type.app_rule
       assumption
       apply ihe2
-      assumption
-      assumption
